\documentclass[../MainPaper.tex]{subfiles}
\begin{document}

\section{Problem}

The output current and mass of the solar panel are both assumed to be dependent on it's area.
\begin{equation}
	I(x_s, y_s) = Iconst * x_s * y_s
\end{equation}
\begin{equation}
	m_s(x_s, y_s) = mconst_s * x_s * y_s
\end{equation}

\noindent The capacity and mass of the Supercap are both assumed to be dependent on it's volume.
\begin{equation}
	C(x_c, y_c, z_c) = Cconst * x_c * y_c * z_c
\end{equation}
\begin{equation}
	m_c(x_c, y_c, z_c) = mconst_c * x_c * y_c * z_c
\end{equation}

\noindent And let's say the mass of the pcb is also dependent on it's area
\begin{equation}
	m_p(x_p, y_p) = mconst_p * x_p * y_p
\end{equation}

\noindent Assuming the current from the solar panel is directly used to increase the voltage in the Supercap:
\begin{equation}
	V(I, t) = \frac{1}{C} I t
\end{equation}
\begin{equation}
	V(x_s, y_s, t) = \frac{1}{C} * ( Iconst * x_s * y_s ) * t 
\end{equation}

\noindent Substituting the equation found for the capacity and voltage of the Supercap gives it's energy:
\begin{equation}
	E(V, C) = \frac{1}{2} C V^2
\end{equation}
\begin{equation}
	E(x_c, y_c, z_c, x_s, y_s, t) = \frac{1}{2} * \frac{1}{Cconst * x_c * y_c * z_c} * (Iconst * x_s * y_s)^2 * t^2
\end{equation}

\noindent Let's assume that all the electrical energy in the supercap is converted to kinetic energy.
\begin{equation}
	E_{elec} = E_{kin}
\end{equation}

\begin{equation}
	E_{kin}(m, v) = \frac{1}{2} m v^2
\end{equation}
\noindent Without any losses the speed is estimated to be:
\begin{equation}
	v(E, m) = \sqrt{\frac{2E}{m}}
\end{equation}

\begin{equation}
	m_{tot} = m_s + m_c + m_p
\end{equation}

\begin{equation}
	v(E, m_{tot}) = \sqrt{\frac{\frac{(Iconst * x_s * y_s)^2 * t^2}{Cconst * x_c * y_c * z_c}}{(mconst_s * x_s * y_s) + (mconst_c * x_c * y_c * z_c) + (mconst_p * x_p * y_p)}}
\end{equation}


\end{document}
	
